examples/mw/MWApp01proof.v
@@ -1,0 +1,80 @@
+Require Import HoareDef MWHeader MWApp0 MWApp1 SimModSem.
+Require Import Coqlib.
+Require Import ImpPrelude.
+Require Import Skeleton.
+Require Import PCM.
+Require Import ModSem Behavior.
+Require Import Relation_Definitions.
+
+(*** TODO: export these in Coqlib or Universe ***)
+Require Import Relation_Operators.
+Require Import RelationPairs.
+From ITree Require Import
+     Events.MapDefault.
+From ExtLib Require Import
+     Core.RelDec
+     Structures.Maps
+     Data.Map.FMapAList.
+
+Require Import HTactics ProofMode.
+
+Set Implicit Arguments.
+
+Local Open Scope nat_scope.
+
+
+
+Section SIMMODSEM.
+
+  Context `{Σ: GRA.t}.
+  Context `{@GRA.inG AppRA Σ}.
+
+  Let W: Type := Any.t * Any.t.
+
+  Let wf: _ -> W -> Prop :=
+    @mk_wf
+      _
+      unit
+      (fun _ _ st_tgt => ((OwnM(AppInitX) ∧ ⌜st_tgt = false↑⌝) ∨ (OwnM(AppRunX) ∧ ⌜st_tgt = true↑⌝))%I)
+  .
+
+  Theorem correct: refines2 [MWApp0.App] [MWApp1.App].
+  Proof.
+    eapply adequacy_local2. econs; ss.
+    i. econstructor 1 with (wf:=wf) (le:=top2); et; swap 2 3.
+    { ss. }
+    { esplits. econs; ss. eapply to_semantic. iIntros "H". iLeft. iSplits; ss. }
+
+    econs; ss.
+    { init. harg. mDesAll. des; clarify. unfold initF, ccallU. steps.
+      mDesOr "INV"; mDesAll; des; clarify.
+      2: { mAssertPure False; ss. iCombine "INV A" as "A". iOwnWf "A" as WF0. admit "ez". }
+      steps. rewrite Any.upcast_downcast in *. clarify. steps.
+      hcall _ _ _ with "INV"; auto.
+      { esplits; ss. }
+      steps. mDesAll; clarify. mDesOr "INV1"; mDesAll; clarify.
+      2: { mAssertPure False; ss. iCombine "INV1 A" as "A". iOwnWf "A" as WF0. admit "ez". }
+      rewrite _UNWRAPU. steps.
+      mAssert _ with "*".
+      { iCombine "A" "INV1" as "A". iApply (OwnM_Upd with "A").
+        instantiate (1:=AppRun ⋅ AppRunX). admit "ez". }
+      hret _; ss.
+      { iMod "A1". iDestruct "A1" as "[A B]". iFrame. iSplits; ss; et. }
+    }
+    econs; ss.
+    { init. harg. mDesAll. des; clarify. unfold runF, ccallU. steps.
+      mDesOr "INV"; mDesAll; des; clarify.
+      1: { mAssertPure False; ss. iCombine "INV A" as "A". iOwnWf "A" as WF0. admit "ez". }
+      steps. rewrite Any.upcast_downcast in *. clarify. steps.
+      hcall _ _ _ with "INV"; auto.
+      { esplits; ss. }
+      steps. mDesAll; clarify. mDesOr "INV1"; mDesAll; clarify.
+      1: { mAssertPure False; ss. iCombine "INV1 A" as "A". iOwnWf "A" as WF0. admit "ez". }
+      rewrite _UNWRAPU. steps.
+      hret _; ss.
+      { iFrame. iSplits; ss; et. }
+    }
+  Unshelve. all: ss. all: try exact 0.
+  Qed.
+
+End SIMMODSEM.
